theories/trace_helpers.v
@@ -1,0 +1,74 @@
+From intensional.heap_lang Require Import lang notation.
+From intensional Require Import stdpp_extra tactics.
+Set Default Proof Using "Type".
+Implicit Types t : list val.
+
+Definition check_tag (tag: string) (v: val) :=
+  match v with
+  | (# (LitTag tag'), _)%V => String.eqb tag tag'
+  | _ => false
+  end.
+
+Lemma check_tag_in_tags tag v t :
+  check_tag tag v = true →
+  v ∈ t →
+  tag ∈ tags t.
+Proof.
+  revert tag v. induction t as [|v' t].
+  { intros ? ? ?. inversion 1. }
+  { intros * H1 [->|H2]%elem_of_cons. cbn.
+    { unfold check_tag in H1. repeat case_match; simplify_eq; eauto.
+      apply String.eqb_eq in H1. subst. constructor. }
+    { cbn. apply elem_of_app. right. eapply IHt; eauto. } }
+Qed.
+
+Lemma fresh_tag_nocheck t tag :
+  tag ∉ tags t →
+  Forall (λ v, ¬ check_tag tag v) t.
+Proof.
+  induction t as [|v t]. done.
+  cbn. repeat case_match; eauto; simplify_eq.
+  intros [? ?]%not_elem_of_cons. apply Forall_cons. split; eauto.
+  unfold check_tag. intros Heq%Is_true_eq_true.
+  by apply String.eqb_eq in Heq as ->.
+Qed.
+
+Lemma not_check_tag_iff (tag tag':string) v :
+  ¬ check_tag tag (#tag', v)%V ↔ tag ≠ tag'.
+Proof.
+  unfold check_tag. split; intros HH1 HH2; apply HH1.
+  { subst. rewrite String.eqb_refl //. }
+  { apply Is_true_eq_true, String.eqb_eq in HH2. auto. }
+Qed.
+
+Lemma check_tag_iff (tag tag':string) v :
+  check_tag tag (#tag', v)%V = true ↔ tag = tag'.
+Proof.
+  unfold check_tag. split; intros HH.
+  { apply String.eqb_eq in HH. auto. }
+  { subst. rewrite String.eqb_refl //. }
+Qed.
+
+Lemma filter_check_single_tag_neq (tag tag':string) v :
+  tag ≠ tag' →
+  filter (λ v, check_tag tag v) [(#tag', v)%V] = [].
+Proof.
+  intros. apply filter_is_nil. repeat constructor.
+  by apply not_check_tag_iff.
+Qed.
+
+Lemma filter_check_single_tag_eq (tag:string) v :
+  filter (λ v, check_tag tag v) [(#tag, v)%V] = [(#tag, v)%V].
+Proof.
+  intros. apply filter_Forall_id. repeat constructor.
+  by apply Is_true_eq_left, check_tag_iff.
+Qed.
+
+Lemma tags_app t u : tags (t ++ u) = tags t ++ tags u.
+Proof.
+  induction t as [|v t].
+  { cbn [tags]. done. }
+  { cbn. case_match. all: try rewrite IHt //. subst.
+    repeat case_match; auto. }
+Qed.
+
